cbor_compare, cbor_compare_correct'

src/cbor/impl/CBOR.Spec.fst
@@ -46,6 +46,176 @@ let deterministically_encoded_cbor_map_key_order_assoc_ext
   m1 m2 ext
 = CBOR.Spec.Format.deterministically_encoded_cbor_map_key_order_assoc_ext m1 m2 ext
 
+let int_compare (x1 x2: int) : Tot int =
+  if x1 < x2
+  then -1
+  else if x1 = x2
+  then 0
+  else 1
+
+let rec bytes_lex_compare
+  (s1 s2: Seq.seq U8.t)
+: Tot int
+  (decreases (Seq.length s1))
+= if Seq.length s1 = 0 || Seq.length s2 = 0
+  then int_compare (Seq.length s1) (Seq.length s2)
+  else
+    let c = int_compare (U8.v (Seq.index s1 0)) (U8.v (Seq.index s2 0)) in
+    if c = 0
+    then bytes_lex_compare (Seq.tail s1) (Seq.tail s2)
+    else c
+
+let rec bytes_lex_compare_correct
+  (s1 s2: Seq.seq U8.t)
+: Lemma
+  (ensures (bytes_lex_compare s1 s2 == LowParse.Spec.SeqBytes.bytes_lex_compare s1 s2))
+  (decreases (Seq.length s1))
+  [SMTPat (bytes_lex_compare s1 s2)]
+= if Seq.length s1 = 0 || Seq.length s2 = 0
+  then ()
+  else bytes_lex_compare_correct (Seq.tail s1) (Seq.tail s2)
+
+let deterministically_encoded_cbor_map_key_order_spec
+  (x1 x2: raw_data_item)
+: Lemma
+  (Ghost.reveal deterministically_encoded_cbor_map_key_order x1 x2 == (bytes_lex_compare (serialize_cbor x1) (serialize_cbor x2) < 0))
+= ()
+
+let rec cbor_compare
+  (x1 x2: raw_data_item)
+: Tot int
+  (decreases x1)
+= let ty1 = get_major_type x1 in
+  let ty2 = get_major_type x2 in
+  let c = int_compare (U8.v ty1) (U8.v ty2) in
+  if c <> 0
+  then c
+  else if ty1 = major_type_uint64 || ty1 = major_type_neg_int64
+  then int_compare (U64.v (Int64?.v x1)) (U64.v (Int64?.v x2))
+  else if ty1 = major_type_simple_value
+  then int_compare (U8.v (Simple?.v x1)) (U8.v (Simple?.v x2))
+  else if ty1 = major_type_byte_string || ty1 = major_type_text_string
+  then
+    let c = int_compare (Seq.length (String?.v x1)) (Seq.length (String?.v x2)) in
+    if c <> 0
+    then c
+    else bytes_lex_compare (String?.v x1) (String?.v x2)
+  else if ty1 = major_type_tagged
+  then
+    let c = int_compare (U64.v (Tagged?.tag x1)) (U64.v (Tagged?.tag x2)) in
+    if c <> 0
+    then c
+    else cbor_compare (Tagged?.v x1) (Tagged?.v x2)
+  else if ty1 = major_type_array
+  then
+    let c = int_compare (List.Tot.length (Array?.v x1)) (List.Tot.length (Array?.v x2)) in
+    if c <> 0
+    then c
+    else cbor_compare_array (Array?.v x1) (Array?.v x2)
+  else if ty1 = major_type_map
+  then
+    let c = int_compare (List.Tot.length (Map?.v x1)) (List.Tot.length (Map?.v x2)) in
+    if c <> 0
+    then c
+    else cbor_compare_map (Map?.v x1) (Map?.v x2)
+  else false_elim ()
+
+and cbor_compare_array
+  (x1 x2: list raw_data_item)
+: Pure int
+    (requires (List.Tot.length x1 == List.Tot.length x2))
+    (ensures (fun _ -> True))
+    (decreases x1)
+= match x1, x2 with
+  | [], [] -> 0
+  | a1 :: q1, a2 :: q2 ->
+    let c = cbor_compare a1 a2 in
+    if c <> 0
+    then c
+    else cbor_compare_array q1 q2
+
+and cbor_compare_map
+  (x1 x2: list (raw_data_item & raw_data_item))
+: Pure int
+    (requires (List.Tot.length x1 == List.Tot.length x2))
+    (ensures (fun _ -> True))
+    (decreases x1)
+= match x1, x2 with
+  | [], [] -> 0
+  | a1 :: q1, a2 :: q2 ->
+    let c = cbor_compare (fst a1) (fst a2) in
+    if c <> 0
+    then c
+    else
+      let c = cbor_compare (snd a1) (snd a2) in
+      if c <> 0
+      then c
+      else cbor_compare_map q1 q2
+
+#push-options "--z3rlimit 32"
+
+#restart-solver
+let rec cbor_compare_correct'
+  (x1 x2: raw_data_item)
+: Lemma
+  (ensures (cbor_compare x1 x2 == bytes_lex_compare (serialize_cbor x1) (serialize_cbor x2)))
+  (decreases x1)
+= let ty1 = get_major_type x1 in
+  if LowParse.Spec.SeqBytes.byte_compare (get_major_type x1) (get_major_type x2) <> 0
+  then serialized_lex_compare_major_type_intro x1 x2
+  else if ty1 = major_type_uint64 || ty1 = major_type_neg_int64
+  then serialized_lex_compare_int64 ty1 (Int64?.v x1) (Int64?.v x2)
+  else if ty1 = major_type_simple_value
+  then serialized_lex_compare_simple_value (Simple?.v x1) (Simple?.v x2)
+  else if ty1 = major_type_byte_string || ty1 = major_type_text_string
+  then serialized_lex_compare_string ty1 (U64.uint_to_t (Seq.length (String?.v x1))) (String?.v x1) (U64.uint_to_t (Seq.length (String?.v x2))) (String?.v x2)
+  else if ty1 = major_type_tagged
+  then begin
+    serialized_lex_compare_tagged (Tagged?.tag x1) (Tagged?.v x1) (Tagged?.tag x2) (Tagged?.v x2);
+    cbor_compare_correct' (Tagged?.v x1) (Tagged?.v x2)
+  end
+  else if ty1 = major_type_array
+  then begin
+    serialized_lex_compare_array (U64.uint_to_t (List.Tot.length (Array?.v x1))) (Array?.v x1) (U64.uint_to_t (List.Tot.length (Array?.v x2))) (Array?.v x2);
+    if List.Tot.length (Array?.v x1) = List.Tot.length (Array?.v x2)
+    then cbor_compare_array_correct (Array?.v x1) (Array?.v x2)
+  end
+  else if ty1 = major_type_map
+  then begin
+    serialized_lex_compare_map (U64.uint_to_t (List.Tot.length (Map?.v x1))) (Map?.v x1) (U64.uint_to_t (List.Tot.length (Map?.v x2))) (Map?.v x2);
+    if List.Tot.length (Map?.v x1) = List.Tot.length (Map?.v x2)
+    then cbor_compare_map_correct (Map?.v x1) (Map?.v x2)
+  end
+  else assert False
+
+and cbor_compare_array_correct
+  (x1 x2: list raw_data_item)
+: Lemma
+  (requires (List.Tot.length x1 == List.Tot.length x2))
+  (ensures (cbor_compare_array x1 x2 == LowParse.Spec.Sorted.lex_compare (serialized_lex_compare serialize_raw_data_item) x1 x2))
+  (decreases x1)
+= match x1, x2 with
+  | a1 :: q1, a2 :: q2 ->
+    cbor_compare_correct' a1 a2;
+    cbor_compare_array_correct q1 q2
+  | _ -> ()
+
+and cbor_compare_map_correct
+  (x1 x2: list (raw_data_item & raw_data_item))
+: Lemma
+  (requires (List.Tot.length x1 == List.Tot.length x2))
+  (ensures (cbor_compare_map x1 x2 == LowParse.Spec.Sorted.lex_compare (serialized_lex_compare (LowParse.Spec.Combinators.serialize_nondep_then serialize_raw_data_item serialize_raw_data_item)) x1 x2))
+  (decreases x1)
+= match x1, x2 with
+  | a1 :: q1, a2 :: q2 ->
+    cbor_compare_correct' (fst a1) (fst a2);
+    cbor_compare_correct' (snd a1) (snd a2);
+    serialized_lex_compare_nondep_then serialize_raw_data_item serialize_raw_data_item a1 a2;
+    cbor_compare_map_correct q1 q2
+  | _ -> ()
+
+#pop-options
+
 let deterministically_encoded_cbor_map_key_order_major_type_intro
   v1 v2
 = CBOR.Spec.Format.deterministically_encoded_cbor_map_key_order_major_type_intro v1 v2
